More progress in generators

src/Generators.v
@@ -108,3 +108,129 @@ Next Obligation.
   exists r1; auto.
 Defined.
 
+(* Generator specific sample of a single input. *)
+Definition sample1 (A : Type) (g : G A) : A :=
+    match g with
+      | MkGen m =>
+        let rnd := newRandomSeed in
+        m 10 rnd
+    end.
+
+(* Generator specific - shrinking support. *)
+Definition promote {A : Type} (m : Rose (G A)) : G (Rose A) :=
+    MkGen (fun n r => fmapRose (fun g => run g n r) m).
+
+(* Generator specific - coarbitrary support. *)
+Definition variant {A : Type} (p : SplitPath) (g : G A) : G A := 
+    match g with 
+      | MkGen f => MkGen (fun n r => f n (varySeed p r))
+    end.
+  
+Definition reallyUnsafeDelay {A : Type} : G (G A -> A) :=
+    MkGen (fun r n g => (match g with MkGen f => f r n end)).
+  
+Definition reallyUnsafePromote {r A : Type} (m : r -> G A) : G (r -> A) :=
+    (bindGen reallyUnsafeDelay (fun eval => 
+                                  returnGen (fun r => eval (m r)))).
+
+Lemma promoteVariant :
+    forall {A B : Type} (a : A) (f : A -> SplitPath) (g : G B) size
+      (r r1 r2 : RandomSeed),
+      randomSplit r = (r1, r2) ->
+      run (reallyUnsafePromote (fun a => variant (f a) g)) size r a =
+      run g size (varySeed (f a) r1).
+Proof.
+    move => A B a p g size r r1 r2 H.
+    rewrite /reallyUnsafePromote /variant.
+    destruct g. rewrite /= H. by [].
+Qed.
+
+Lemma semPromote A (m : Rose (G A)) :
+    semProd (promote m) <-->
+    codom2 (fun size seed => fmapRose (fun g => run g size seed) m).
+Proof. by rewrite /codom2 curry_codom2l. Qed.
+
+Lemma semPromoteSize (A : Type) (m : Rose (G A)) n :
+    semGenSize (promote m) n <-->
+               codom (fun seed => fmapRose (fun g => run g n seed) m).
+Proof. by []. Qed.
+
+Lemma runPromote A (m : Rose (G A)) seed size :
+    run (promote m) seed size = fmapRose (fun (g : G A) => run g seed size) m.
+Proof. by []. Qed.
+
+
+(* Generator specific - choose and its semantics. *)
+Definition choose {A : Type} `{ChoosableFromInterval A} (range : A * A) : G A :=
+    MkGen (fun _ r => fst (randomR range r)).
+
+
+Lemma semChooseSize A `{ChoosableFromInterval A} (a1 a2 : A) :
+    RandomQC.leq a1 a2 ->
+    forall size, semGenSize (choose (a1,a2)) size <-->
+                       [set a | RandomQC.leq a1 a && RandomQC.leq a a2].
+Proof. by move=> /= le_a1a2 m n; rewrite (randomRCorrect n a1 a2). Qed.
+  
+Instance chooseUnsized {A} `{RandomQC.ChoosableFromInterval A} (a1 a2 : A) :
+    Unsized (choose (a1, a2)).
+Proof. by []. Qed.
+  
+Lemma semChoose A `{RandomQC.ChoosableFromInterval A} (a1 a2 : A) :
+    RandomQC.leq a1 a2 ->
+    (semProd (choose (a1,a2)) <--> [set a | RandomQC.leq a1 a && RandomQC.leq a a2]).
+Proof.
+  move=> /= le_a1a2. rewrite <- (unsized_alt_def 1).
+  move => m /=. rewrite (randomRCorrect m a1 a2) //.
+Qed.
+
+  Definition thunkGen {A} (f : unit -> G A) : G A :=
+    MkGen (fun n r => run (f tt) n r).
+
+  Lemma semThunkGenSize {A} (f : unit -> G A) s :
+    semProdSize (thunkGen f) s <--> semProdSize (f tt) s.
+  Proof.
+    split; intros [r Hr]; exists r; simpl in *; assumption.
+  Qed.
+
+  Lemma semThunkGen {A} (f : unit -> G A) :
+    semProd (thunkGen f) <--> semProd (f tt).
+  Proof.
+    split; intros [r Hr]; exists r; simpl in *; assumption.
+  Qed.
+
+  Instance thunkGenUnsized {A} (f : unit -> G A)
+          `{@Unsized _ _ ProducerGen (f tt)} : Unsized (thunkGen f).
+  Proof.
+    intros s1 s2.
+    Set Printing All.
+    do 2 rewrite semThunkGenSize.
+    apply unsized.
+  Qed.
+
+  Instance thunkGenSizeMonotonic {A} (f : unit -> G A)
+          `{@SizeMonotonic _ _ ProducerGen (f tt)} : SizeMonotonic (thunkGen f).
+  Proof.
+    intros s1 s2 Hs.
+    do 2 rewrite semThunkGenSize.
+    by apply monotonic.
+  Qed.
+
+  Instance thunkGenSizeMonotonicOpt {A} (f : unit -> G (option A))
+          `{@SizeMonotonicOpt _ _ ProducerGen (f tt)} : SizeMonotonicOpt (thunkGen f).
+  Proof.
+    intros s1 s2 Hs. unfold semProdSizeOpt.
+    do 2 rewrite semThunkGenSize.
+    by apply monotonicOpt.
+  Qed.
+
+  Instance thunkGenSizeAntiMonotonicNone {A} (f : unit -> G (option A))
+          `{@SizeAntiMonotonicNone _ _ ProducerGen (f tt)} : SizeAntiMonotonicNone (thunkGen f).
+  Proof.
+    intros s1 s2 Hs.
+    do 2 rewrite semThunkGenSize.
+    by apply monotonicNone.
+  Qed.
+
+
+
+
